Some progress in folded vs unfolded. Save to fix a small bug in floyd.

mc_reify/verif_nest3.v
@@ -50,49 +50,99 @@ Definition multi_command_spec :=
                           ((Int.add i122 (Int.repr 4), Int.add i121 (Int.repr 3)),
                            (Int.add i112 (Int.repr 2), Int.add i111 (Int.repr 1))))) p).
 
-(* The following specs are not in super canonical form. *)
-Definition get_spec2 :=
- DECLARE _get
-  WITH v : reptype' t_struct_c, p: val
-  PRE  [] 
-        PROP  ()
-        LOCAL (var _p t_struct_c p)
-        SEP   (`(data_at Ews t_struct_c (repinj _ v)) (eval_var _p t_struct_c))
-  POST [ tint ]
-        PROP  ()
-        LOCAL (`(eq p) (eval_var _p t_struct_c); 
-               `(eq (Vint (snd (snd (snd v))))) (eval_id 1%positive))
-        SEP   (`(data_at Ews t_struct_c (repinj _ v)) (eval_var _p t_struct_c)).
-
-Definition get_spec3 :=
- DECLARE _get
-  WITH v : reptype' t_struct_c, p: val
-  PRE  [] 
-        PROP  ()
-        LOCAL ()
-        SEP   (`(data_at Ews t_struct_c (repinj _ v)) (eval_var _p t_struct_c))
-  POST [ tint ]
-        PROP  ()
-        LOCAL (`(eq (Vint (snd (snd (snd v))))) (eval_id 1%positive))
-        SEP   (`(data_at Ews t_struct_c (repinj _ v)) (eval_var _p t_struct_c)).
-
-Definition set_spec2 :=
- DECLARE _set
-  WITH i : int, v : reptype' t_struct_c
-  PRE  [ _i OF tint ] 
-         PROP () LOCAL(temp _i (Vint i))
-        SEP(`(data_at Ews t_struct_c (repinj _ v)) (eval_var _p t_struct_c))
+Definition multi_command_s_spec :=
+ DECLARE _multi_command_s
+  WITH p0: val,
+       p1: val,
+       p2: val,
+       p3: val,
+       p4: val,
+       p5: val,
+       p6: val,
+       p7: val
+  PRE  []
+        PROP ()
+        LOCAL(var _p0 t_struct_c p0;
+              var _p1 t_struct_c p1;
+              var _p2 t_struct_c p2;
+              var _p3 t_struct_c p3;
+              var _p4 t_struct_c p4;
+              var _p5 t_struct_c p5;
+              var _p6 t_struct_c p6;
+              var _p7 t_struct_c p7)
+        SEP(`(data_at Ews tint (Vint (Int.repr 0)) p0);
+            `(data_at Ews tint (Vint (Int.repr 0)) p1);
+            `(data_at Ews tint (Vint (Int.repr 0)) p2);
+            `(data_at Ews tint (Vint (Int.repr 0)) p3);
+            `(data_at Ews tint (Vint (Int.repr 0)) p4);
+            `(data_at Ews tint (Vint (Int.repr 0)) p5);
+            `(data_at Ews tint (Vint (Int.repr 0)) p6);
+            `(data_at Ews tint (Vint (Int.repr 0)) p7))
   POST [ tvoid ]
-        `(data_at Ews t_struct_c (repinj _ (update222 i v))) (eval_var _p t_struct_c).
+        PROP ()
+        LOCAL(var _p0 t_struct_c p0;
+              var _p1 t_struct_c p1;
+              var _p2 t_struct_c p2;
+              var _p3 t_struct_c p3;
+              var _p4 t_struct_c p4;
+              var _p5 t_struct_c p5;
+              var _p6 t_struct_c p6;
+              var _p7 t_struct_c p7)
+        SEP(`(data_at Ews tint (Vint (Int.repr 0)) p0);
+            `(data_at Ews tint (Vint (Int.repr 0)) p1);
+            `(data_at Ews tint (Vint (Int.repr 0)) p2);
+            `(data_at Ews tint (Vint (Int.repr 0)) p3);
+            `(data_at Ews tint (Vint (Int.repr 4)) p4);
+            `(data_at Ews tint (Vint (Int.repr 3)) p5);
+            `(data_at Ews tint (Vint (Int.repr 2)) p6);
+            `(data_at Ews tint (Vint (Int.repr 1)) p7)).
 
 Definition Vprog : varspecs := (_p, t_struct_c)::nil.
 
 Definition Gprog : funspecs := 
-    get_spec::set_spec::multi_command_spec::nil.
+    multi_command_s_spec::multi_command_spec::nil.
 
 Require Import Timing.
 Clear Timing Profile.
 
+Lemma body_multi_command_s: semax_body Vprog Gprog f_multi_command_s multi_command_s_spec.
+Proof.
+  start_function.
+start_timer "Folded".
+eapply semax_seq'.
+eapply semax_seq'.
++
+hoist_later_in_pre.
+
+eapply sc_set_load_store.semax_SC_field_load with (e1 := (Evar _p0 tint)) (efs := nil) (tts := nil)
+(gfs := nil) (gfs0 := nil) (gfs1 := nil) (e := Struct_env) (t_root := tint) (n := 0%nat) (lr := LLLL).
+reflexivity.
+reflexivity.
+reflexivity.
+Locate legal_nested_efield.
+Print compute_lr.
+reflexivity.
+
+
+
+
+
+  forward.forward. [entailer! | solve_legal_nested_field_in_entailment' |].
+  simpl upd_reptype.
+  forward.forward; [entailer! | solve_legal_nested_field_in_entailment' |].
+  simpl upd_reptype.
+  forward.forward; [entailer! | solve_legal_nested_field_in_entailment' |].
+  forward.forward; [entailer! | solve_legal_nested_field_in_entailment' |].
+  simpl upd_reptype.
+  forward.forward; [entailer! | solve_legal_nested_field_in_entailment' |].
+  forward.forward; [entailer! | solve_legal_nested_field_in_entailment' |].
+  simpl upd_reptype.
+  forward.forward; [entailer! | solve_legal_nested_field_in_entailment' |].
+  forward.forward; [entailer! | solve_legal_nested_field_in_entailment' |].
+  simpl upd_reptype.
+stop_timer "Folded".
+  forward.forward. (* return *)
+Qed.
 Lemma body_multi_command: semax_body Vprog Gprog f_multi_command multi_command_spec.
 Proof.
   start_function.
